-

main/SortingFun.v
@@ -3377,7 +3377,291 @@ apply (sorted_unique Href Hant Htra). {
 }
 Qed.
 
-(* isort rank *)
+
+(* isort_rank: like isort but return the rank of what have been
+   sorted; its result, when applied to the initial list as an
+   operator, returns the sorted list  *)
+
+Fixpoint isort_rank_insert {A B} (rel : A → A → bool) (f : B → A) ia lrank :=
+  match lrank with
+  | [] => [ia]
+  | ib :: l =>
+      if rel (f ia) (f ib) then ia :: lrank
+      else ib :: isort_rank_insert rel f ia l
+  end.
+
+Fixpoint isort_rank_loop {A} (rel : A → A → bool) f lrank (l : list A) :=
+  match l with
+  | [] => lrank
+  | _ :: l' =>
+      isort_rank_loop rel f (isort_rank_insert rel f (length lrank) lrank) l'
+  end.
+
+Definition isort_rank {A} (rel : A → A → bool) l :=
+  match l with
+  | [] => []
+  | d :: _ => isort_rank_loop rel (λ i, nth i l d) [] l
+  end.
+
+(*
+Compute (let l := [2;7;1] in isort_rank Nat.leb l).
+Compute (let l := [5;10;2;7;0] in isort_rank Nat.leb l).
+Compute (let l := [5;2;2;7;0] in isort_rank Nat.leb l).
+Compute (let l := [5;2;2;7;0] in isort_rank Nat.ltb l).
+*)
+
+Theorem isort_rank_insert_length : ∀ A B rel (f : B → A) ia lrank,
+  length (isort_rank_insert rel f ia lrank) = S (length lrank).
+Proof.
+intros.
+induction lrank as [| ib]; [ easy | cbn ].
+destruct (rel (f ia) (f ib)); [ easy | cbn ].
+now rewrite IHlrank.
+Qed.
+
+Theorem isort_rank_loop_length : ∀ A rel (f : _ → A) lrank l,
+  length (isort_rank_loop rel f lrank l) = length lrank + length l.
+Proof.
+intros.
+revert lrank.
+induction l as [| b]; intros; [ easy | cbn ].
+rewrite IHl.
+rewrite isort_rank_insert_length.
+apply Nat.add_succ_comm.
+Qed.
+
+Theorem isort_rank_length : ∀ A rel (l : list A),
+  length (isort_rank rel l) = length l.
+Proof.
+intros.
+unfold isort_rank.
+destruct l as [| d]; [ easy | ].
+remember (d :: l) as l' eqn:Hl'.
+clear l Hl'.
+rename l' into l.
+apply isort_rank_loop_length.
+Qed.
+
+Theorem isort_rank_insert_nth_indep : ∀ A rel (d d' : A) ia lrank l_ini,
+  ia < length l_ini
+  → (∀ i, i ∈ lrank → i < length l_ini)
+  → isort_rank_insert rel (λ i : nat, nth i l_ini d) ia lrank =
+    isort_rank_insert rel (λ i : nat, nth i l_ini d') ia lrank.
+Proof.
+intros * Hia Hini.
+induction lrank as [| ib]; [ easy | ].
+cbn - [ nth ].
+specialize (Hini ib (or_introl eq_refl)) as Hib.
+rewrite (nth_indep _ _ d' Hia).
+rewrite (nth_indep _ _ d' Hib).
+remember (rel (nth ia l_ini d') (nth ib l_ini d')) as x eqn:Hx.
+symmetry in Hx.
+destruct x; [ easy | ].
+f_equal.
+apply IHlrank.
+intros i Hi.
+apply Hini.
+now right.
+Qed.
+
+Theorem in_isort_rank_insert : ∀ A B rel (f : B → A) ia lrank i,
+  i ∈ isort_rank_insert rel f ia lrank
+  → i ∈ ia :: lrank.
+Proof.
+intros * Hil.
+induction lrank as [| ib]; [ easy | ].
+cbn in Hil.
+destruct (rel (f ia) (f ib)); [ easy | ].
+destruct Hil as [Hil| Hil]; [ now subst i; right; left | ].
+specialize (IHlrank Hil).
+destruct IHlrank as [Hi| Hi]; [ now subst i; left | now right; right ].
+Qed.
+
+Theorem isort_rank_loop_nth_indep : ∀ A rel (d d' : A) lrank l_ini l,
+  length lrank + length l ≤ length l_ini
+  → (∀ i, i ∈ lrank → i < length l_ini)
+  → isort_rank_loop rel (λ i, nth i l_ini d) lrank l =
+    isort_rank_loop rel (λ i, nth i l_ini d') lrank l.
+Proof.
+intros * Hia Hil.
+revert lrank Hia Hil.
+induction l as [| b]; intros; [ easy | ].
+cbn - [ nth ] in Hia |-*.
+rewrite isort_rank_insert_nth_indep with (d' := d'); [ | flia Hia | easy ].
+rewrite <- Nat.add_succ_comm in Hia.
+rewrite IHl; [ easy | now rewrite isort_rank_insert_length | ].
+intros i Hi.
+apply in_isort_rank_insert in Hi.
+destruct Hi as [Hi| Hi]; [ subst i; flia Hia | ].
+now apply Hil.
+Qed.
+
+Theorem isort_rank_insert_ub : ∀ A (rel : A → _) ia lrank f i n,
+  ia < n
+  → (∀ i, i ∈ lrank → i < n)
+  → nth i (isort_rank_insert rel f ia lrank) 0 < n.
+Proof.
+intros * Hia Hn.
+revert i.
+induction lrank as [| ib]; intros. {
+  destruct i; [ easy | cbn ].
+  rewrite match_id; flia Hia.
+}
+cbn - [ nth ].
+remember (rel (f ia) (f ib)) as x eqn:Hx.
+symmetry in Hx.
+destruct x. {
+  destruct i; [ easy | ].
+  rewrite List_nth_succ_cons.
+  destruct (lt_dec i (length (ib :: lrank))) as [Hii| Hii]. 2: {
+    apply Nat.nlt_ge in Hii.
+    rewrite nth_overflow; [ flia Hia | easy ].
+  }
+  now apply Hn, nth_In.
+} {
+  destruct i; [ now cbn; apply Hn; left | cbn ].
+  apply IHlrank.
+  intros j Hj.
+  now apply Hn; right.
+}
+Qed.
+
+Theorem isort_rank_loop_ub : ∀ A (rel : A → _) f lrank l i,
+  length lrank + length l ≠ 0
+  → (∀ i, i ∈ lrank → i < length lrank + length l)
+  → nth i (isort_rank_loop rel f lrank l) 0 <
+    length lrank + length l.
+Proof.
+intros * Hlz Hil.
+destruct (lt_dec i (length lrank + length l)) as [Hir| Hir]. 2: {
+  apply Nat.nlt_ge in Hir.
+  rewrite nth_overflow; [ | now rewrite isort_rank_loop_length ].
+  now apply Nat.neq_0_lt_0.
+}
+clear Hlz.
+revert lrank Hil Hir.
+induction l as [| b]; intros. {
+  rewrite Nat.add_0_r in Hir.
+  now apply Hil, nth_In.
+}
+cbn in Hir |-*.
+rewrite <- Nat.add_succ_comm in Hir |-*.
+specialize (in_isort_rank_insert) as H1.
+specialize (H1 A nat rel f (length lrank) lrank).
+remember (isort_rank_insert rel f (length lrank) lrank) as lr' eqn:Hlr'.
+specialize isort_rank_insert_length as H2.
+specialize (H2 A nat rel f (length lrank) lrank).
+rewrite <- Hlr' in H2.
+rewrite <- H2 in Hir |-*.
+apply IHl; [ | easy ].
+intros j Hj.
+rewrite H2, Nat.add_succ_comm.
+rewrite Hlr' in Hj.
+apply in_isort_rank_insert in Hj.
+destruct Hj as [Hj| Hj]; [ subst j; flia | ].
+now apply Hil.
+Qed.
+
+Theorem isort_rank_ub : ∀ A rel (l : list A) i,
+  l ≠ [] → nth i (isort_rank rel l) 0 < length l.
+Proof.
+intros * Hlz.
+destruct l as [| ia]; [ easy | clear Hlz ].
+cbn - [ nth ].
+apply isort_rank_loop_ub; [ easy | ].
+intros j Hj.
+destruct Hj; [ now subst j; cbn | easy ].
+Qed.
+
+Theorem in_isort_rank_lt : ∀ A (rel : A → _) l i,
+  i ∈ isort_rank rel l → i < length l.
+Proof.
+intros * Hi.
+apply (In_nth _ _ 0) in Hi.
+destruct Hi as (j & Hjl & Hji).
+rewrite isort_rank_length in Hjl.
+rewrite <- Hji.
+apply isort_rank_ub.
+now intros H; subst l.
+Qed.
+
+Theorem NoDup_isort_rank_insert : ∀ A (d : A) rel l_ini ia lrank,
+  NoDup (ia :: lrank)
+  → NoDup (isort_rank_insert rel (λ k : nat, nth k l_ini d) ia lrank).
+Proof.
+intros * Hnd.
+revert ia Hnd.
+induction lrank as [| ib]; intros. {
+  cbn; constructor; [ easy | constructor ].
+}
+cbn.
+destruct (rel (nth ia l_ini d) (nth ib l_ini d)); [ easy | ].
+apply NoDup_cons_iff in Hnd.
+destruct Hnd as (Hia, Hnd).
+apply NoDup_cons_iff in Hnd.
+destruct Hnd as (Hib, Hnd).
+apply NoDup_cons. 2: {
+  apply IHlrank.
+  apply NoDup_cons_iff.
+  split; [ | easy ].
+  now intros H; apply Hia; right.
+}
+intros Hib'.
+apply in_isort_rank_insert in Hib'.
+destruct Hib' as [Hib'| Hib']; [ | easy ].
+subst ib; apply Hia.
+now left.
+Qed.
+
+Theorem NoDup_isort_rank_loop : ∀ A d rel l_ini (l : list A) lrank,
+  NoDup lrank
+  → AllLt lrank (length lrank)
+  → NoDup (isort_rank_loop rel (λ k, nth k l_ini d) lrank l).
+Proof.
+intros * Hnd Halt.
+revert lrank Hnd Halt.
+induction l as [| a]; intros; [ easy | cbn ].
+apply IHl.
+apply NoDup_isort_rank_insert. 2: {
+  rewrite isort_rank_insert_length.
+  intros i Hi.
+  apply in_isort_rank_insert in Hi.
+  destruct Hi as [Hi| Hi]; [ now rewrite Hi | ].
+  specialize (Halt _ Hi) as H1.
+  flia H1.
+}
+apply NoDup_cons_iff.
+split; [ | easy ].
+intros H.
+specialize (Halt _ H) as H1.
+now apply Nat.lt_irrefl in H1.
+Qed.
+
+Theorem NoDup_isort_rank : ∀ A rel (l : list A), NoDup (isort_rank rel l).
+Proof.
+intros.
+apply (proj2 (NoDup_nth _ 0)).
+rewrite isort_rank_length.
+intros i j Hi Hj Hij.
+destruct l as [| d]; [ easy | ].
+unfold isort_rank in Hij.
+specialize (NoDup_isort_rank_loop d rel (d :: l) (d :: l) (NoDup_nil _)) as H1.
+assert (H : AllLt [] (length ([] : list nat))) by easy.
+specialize (H1 H); clear H.
+specialize (proj1 (NoDup_nth _ 0) H1) as H2.
+rewrite isort_rank_loop_length in H2.
+rewrite Nat.add_0_l in H2.
+apply (H2 i j Hi Hj Hij).
+Qed.
+
+Theorem eq_isort_rank_nil : ∀ A (rel : A → _) l,
+  isort_rank rel l = [] → l = [].
+Proof.
+intros * Hl.
+apply (f_equal length) in Hl.
+rewrite isort_rank_length in Hl.
+now apply length_zero_iff_nil in Hl.
+Qed.
 
 Theorem isort_insert_isort_rank_insert : ∀ A B rel ia (f : B → A) lrank,
   isort_insert rel (f ia) (map f lrank) =
@@ -3388,6 +3672,21 @@ induction lrank as [| ib]; [ easy | cbn ].
 destruct (rel (f ia) (f ib)); [ easy | ].
 cbn; f_equal.
 apply IHlrank.
+Qed.
+
+Theorem nth_isort_rank_insert_of_sorted :
+  ∀ A d (rel : A → _) l_ini n ls,
+  (∀ i, i ∈ ls → rel (nth n l_ini d) (nth i l_ini d) = false)
+  → isort_rank_insert rel (λ j : nat, nth j l_ini d) n ls = ls ++ [n].
+Proof.
+intros * Hls.
+induction ls as [| b]; [ easy | cbn ].
+rewrite Hls; [ | now left ].
+f_equal.
+apply IHls.
+intros j Hj.
+apply Hls.
+now right.
 Qed.
 
 Theorem isort_loop_isort_rank_loop : ∀ A rel d (f : nat → A) lrank l,
